backend/Regalloc.ml
@@ -167,6 +167,8 @@ let rec convert_builtin_arg tyenv = function
   | BA_addrglobal(id, ofs) -> BA_addrglobal(id, ofs)
   | BA_splitlong(hi, lo) ->
       BA_splitlong(convert_builtin_arg tyenv hi, convert_builtin_arg tyenv lo)
+  | BA_addptr(a1, a2) ->
+      BA_addptr(convert_builtin_arg tyenv a1, convert_builtin_arg tyenv a2)
 
 let convert_builtin_res tyenv = function
   | BR r ->
@@ -185,6 +187,10 @@ let rec constrain_builtin_arg a cl =
       let (hi', cl1) = constrain_builtin_arg hi cl in
       let (lo', cl2) = constrain_builtin_arg lo cl1 in
       (BA_splitlong(hi', lo'), cl2)
+  | BA_addptr(a1, a2), _ ->
+      let (a1', cl1) = constrain_builtin_arg a1 cl in
+      let (a2', cl2) = constrain_builtin_arg a2 cl1 in
+      (BA_addptr(a1', a2'), cl2)
   | _, _ -> (a, cl)
 
 let rec constrain_builtin_args al cl =
@@ -335,6 +341,7 @@ let rec vset_addarg a after =
   match a with
   | BA v -> VSet.add v after
   | BA_splitlong(hi, lo) -> vset_addarg hi (vset_addarg lo after)
+  | BA_addptr(a1, a2) -> vset_addarg a1 (vset_addarg a2 after)
   | _ -> after
 
 let vset_addargs al after = List.fold_right vset_addarg al after
@@ -432,8 +439,8 @@ let rec dce_parmove srcs dsts after =
 
 let rec keep_builtin_arg after = function
   | BA v -> VSet.mem v after
-  | BA_splitlong(hi, lo) ->
-      keep_builtin_arg after hi && keep_builtin_arg after lo
+  | BA_splitlong(a1, a2) | BA_addptr(a1, a2) ->
+      keep_builtin_arg after a1 && keep_builtin_arg after a2
   | _ -> true
 
 let dce_instr instr after k =
@@ -855,6 +862,10 @@ let rec reload_arg tospill eqs = function
       let (hi', c1, eqs1) = reload_arg tospill eqs hi in
       let (lo', c2, eqs2) = reload_arg tospill eqs1 lo in
       (BA_splitlong(hi', lo'), c1 @ c2, eqs2)
+  | BA_addptr(a1, a2) ->
+      let (a1', c1, eqs1) = reload_arg tospill eqs a1 in
+      let (a2', c2, eqs2) = reload_arg tospill eqs1 a2 in
+      (BA_addptr(a1', a2'), c1 @ c2, eqs2)
   | a -> (a, [], eqs)
 
 let rec reload_args tospill eqs = function
