test/regression/volatile4.c
@@ -1,0 +1,29 @@
+/* Addressing modes in volatiles */
+
+#include <stdio.h>
+
+volatile int g = 1;
+volatile int b[10];
+
+void test1(volatile int * p)
+{
+  volatile int l;
+  volatile int a[10];
+
+  l = 42;
+  printf ("l = %d\n", l);
+  a[5] = 0xff;
+  printf ("a[5] = %d\n", a[5]);
+  g = 3;
+  printf ("g = %d\n", g);
+  b[2] = -1;
+  printf ("b[2] = %d\n", b[2]);
+  p[1] = 80;
+  printf ("p[1] = %d\n", p[1]);
+}
+
+int main()
+{
+  test1(&b[0]);
+  return 0;
+}
