x86/Machregs.v
@@ -358,9 +358,9 @@ Definition two_address_op (op: operation) : bool :=
 Definition builtin_constraints (ef: external_function) :
                                        list builtin_arg_constraint :=
   match ef with
-  | EF_vload _ => OK_addrany :: nil
-  | EF_vstore _ => OK_addrany :: OK_default :: nil
-  | EF_memcpy _ _ => OK_addrany :: OK_addrany :: nil
+  | EF_vload _ => OK_addressing :: nil
+  | EF_vstore _ => OK_addressing :: OK_default :: nil
+  | EF_memcpy _ _ => OK_addrstack :: OK_addrstack :: nil
   | EF_annot txt targs => map (fun _ => OK_all) targs
   | EF_debug kind txt targs => map (fun _ => OK_all) targs
   | _ => nil
